feat: Created size function to allow Dafny to prove termination

examples/boolean.dfy
@@ -6,13 +6,22 @@ datatype Formula =
 | Not(f: Formula) 
 | Imply(left: Formula, right: Formula)
 
+function size(f: Formula): nat
+{
+    match f
+    case True => 1
+    case False => 1
+    case Not(f) => 1 + size(f)
+    case Imply(l, r) => 2 + size(l) + size(r)
+}
+
 // Dafny cannot prove termination for the last clause
 function eval(f: Formula): bool
-    decreases f
+    decreases size(f)
 {
     match f
     case True => true
     case False => false
     case Not(f) => if (eval(f)) then false else true
-    case Imply(fl, fr) => eval(Not(fl)) || eval(fr)
+    case Imply(l, r) => eval(Not(l)) || eval(r)
 }
